@prefix charme: <http://charme.org#> .
@prefix rdf: <http://www.w3.org/1999/02/22-rdf-syntax-ns#> .
@prefix rdfs: <http://www.w3.org/2000/01/rdf-schema#> .
@prefix skos: <http://www.w3.org/2004/02/skos/core#> .
@prefix owl: <http://www.w3.org/2002/07/owl#> .

charme:SignificantEventTypeScheme a skos:ConceptScheme .

charme:EventType a rdf:type ;
	skos:inScheme charme:SignificantEventTypeScheme ;
	skos:prefLabel "EventType"@en ;
	skos:broader rdf:type ;
	rdfs:comment "Generic significant event type"@en .

charme:ClimateEvent a charme:EventType ;
	skos:inScheme charme:SignificantEventTypeScheme ;
	skos:notation "C"@en ;
	skos:prefLabel "Climate Event"@en ;
	skos:narrower charme:HurricaneEvent ;
	skos:narrower charme:VolcanicEruptionEvent ;
	skos:narrower charme:ElNinoEvent ;
	skos:narrower charme:DroughtEvent ;
	skos:narrower charme:StormEvent ;
	skos:narrower charme:WildfiresEvent ;
	rdfs:comment "Defines the charme technical document type specifications"@en .

charme:climateSubEventConceptScheme a skos:ConceptScheme .

charme:HurricaneEvent a charme:EventType ;
	skos:inScheme charme:climateSubEventConceptScheme ;
	skos:prefLabel "Hurricane event"@en ;
	skos:broader charme:ClimateEvent ;
	rdfs:comment "Hurricane significant event type, a sub-type of ClimateEvent"@en .

charme:VolcanicEruptionEvent a charme:EventType ;
	skos:inScheme charme:climateSubEventConceptScheme ;
	skos:prefLabel "Volcanic Eruption"@en ;
	skos:broader charme:ClimateEvent ;
	rdfs:comment "Volcanic eruption significant event type, a sub-type of ClimateEvent"@en .

charme:ElNinoEvent a charme:EventType ;
        skos:inScheme charme:climateSubEventConceptScheme ;
        skos:prefLabel "El Nino event"@en ;
        skos:broader charme:ClimateEvent ;
        rdfs:comment "El Nino significant event type, a sub-type of ClimateEvent"@en .

charme:DroughtEvent a charme:EventType ;
        skos:inScheme charme:climateSubEventConceptScheme ;
        skos:prefLabel "Drought event"@en ;
        skos:broader charme:ClimateEvent ;
        rdfs:comment "Drought significant event type, a sub-type of ClimateEvent"@en .

charme:StormEvent a charme:EventType ;
        skos:inScheme charme:climateSubEventConceptScheme ;
        skos:prefLabel "Storm event"@en ;
        skos:broader charme:ClimateEvent ;
        rdfs:comment "Storm significant event type, a sub-type of ClimateEvent"@en .

charme:WildfiresEvent a charme:EventType ;
        skos:inScheme charme:climateSubEventConceptScheme ;
        skos:prefLabel "Wildfires event"@en ;
        skos:broader charme:ClimateEvent ;
        rdfs:comment "Wildfires significant event type, a sub-type of ClimateEvent"@en .

charme:SoftwareAndSystemEventConceptScheme a skos:ConceptScheme .

charme:SoftwareAndSystemEvent a charme:EventType ;
	skos:inScheme charme:SoftwareAndSystemEventConceptScheme ;
	skos:notation "S"@en ;
	skos:prefLabel "Software/system event"@en ;
	skos:broader charme:EventType ;
	skos:narrower charme:IfsEvent ;
	skos:narrower charme:SystemEvent ;
	rdfs:comment "Software/system significant event type"@en .

charme:IfsEvent a charme:EventType ;
	skos:inScheme charme:SoftwareAndSystemEventConceptScheme ;
	skos:prefLabel "IFS event"@en ;
	skos:broader charme:SoftwareAndSystemEvent ;
	rdfs:comment "IFS significant event type, a sub-type of SoftwareAndSystemEvent"@en .

charme:SystemEvent a charme:EventType ;
	skos:inScheme charme:SoftwareAndSystemEventConceptScheme ;
	skos:prefLabel "System event"@en ;
	skos:broader charme:SoftwareAndSystemEvent ;
	rdfs:comment "System significant event type, a sub-type of SoftwareAndSystemEvent"@en .


# Data / Observing systems events
charme:DataAndObservingSystemEvents a charme:EventType ;
	skos:inScheme charme:SignificantEventTypeScheme ;
	skos:prefLabel "Data / Observing system events"@en ;
	skos:notation "D"@en ;
	skos:narrower charme:SatelliteEvent ;
	skos:narrower charme:DropsondeEvent ;
	skos:narrower charme:AircraftEvent ;
	skos:narrower charme:BuoyEvent ;
	skos:narrower charme:ShipEvent ;
	skos:narrower charme:LandStationEvent ;
	skos:narrower charme:MobileEvent ;
	skos:narrower charme:AlarmEvent ;
	rdfs:comment "Data / observing system event type"@en .

charme:DataAndObservingSystemEventsConceptScheme a skos:ConceptScheme .

charme:SatelliteEvent a charme:EventType ;
	skos:inScheme charme:DataAndObservingSystemEventsConceptScheme ;
	skos:prefLabel "Data / Observing system events"@en ;
	skos:broader charme:DataAndObservingSystemEvents ;
	rdfs:comment "Satellite event type, a sub-type of Data / observing system event type"@en .

charme:DropsondeEvent a charme:EventType ;
	skos:inScheme charme:DataAndObservingSystemEventsConceptScheme ;
	skos:prefLabel "Dropsonde event"@en ;
	skos:broader charme:DataAndObservingSystemEvents ;
	rdfs:comment "Dropsonde event type, a sub-type of Data / observing system event type"@en .

charme:AircraftEvent a charme:EventType ;
	skos:inScheme charme:DataAndObservingSystemEventsConceptScheme ;
	skos:prefLabel "Aircraft event"@en ;
	skos:broader charme:DataAndObservingSystemEvents ;
	rdfs:comment "Aircraft event type, a sub-type of Data / observing system event type"@en .

charme:BuoyEvent a charme:EventType ;
	skos:inScheme charme:DataAndObservingSystemEventsConceptScheme ;
	skos:prefLabel "Buoy event"@en ;
	skos:broader charme:DataAndObservingSystemEvents ;
	rdfs:comment "Buoy event type, a sub-type of Data / observing system event type"@en .

charme:ShipEvent a charme:EventType ;
	skos:inScheme charme:DataAndObservingSystemEventsConceptScheme ;
	skos:prefLabel "Ship event"@en ;
	skos:broader charme:DataAndObservingSystemEvents ;
	rdfs:comment "Ship event type, a sub-type of Data / observing system event type"@en .

charme:LandStationEvent a charme:EventType ;
	skos:inScheme charme:DataAndObservingSystemEventsConceptScheme ;
	skos:prefLabel "Land station event"@en ;
	skos:broader charme:DataAndObservingSystemEvents ;
	rdfs:comment "Land station event type, a sub-type of Data / observing system event type"@en .

charme:MobileEvent a charme:EventType ;
	skos:inScheme charme:DataAndObservingSystemEventsConceptScheme ;
	skos:prefLabel "Mobile event"@en ;
	skos:broader charme:DataAndObservingSystemEvents ;
	rdfs:comment "Mobile event type, a sub-type of Data / observing system event type"@en .

charme:AlarmEvent a charme:EventType ;
	skos:inScheme charme:DataAndObservingSystemEventsConceptScheme ;
	skos:prefLabel "Alarm event"@en ;
	skos:broader charme:DataAndObservingSystemEvents ;
	rdfs:comment "Alarm event type, a sub-type of Data / observing system event type"@en .


# Operational Event
charme:OperationalEvent a charme:EventType ;
	skos:inScheme charme:SignificantEventTypeScheme ;
	skos:prefLabel "Data / Observing system events"@en ;
	skos:notation "O"@en ;
	skos:broader charme:EventType ;
	rdfs:comment "Operational event type"@en .

# - Operational event sub-scheme would go here -

