@prefix charme: <http://purl.org/voc/charme#> .
@prefix dc: <http://purl.org/dc/terms/> .
@prefix rdf: <http://www.w3.org/1999/02/22-rdf-syntax-ns#> .
@prefix rdfs: <http://www.w3.org/2000/01/rdf-schema#> .
@prefix skos: <http://www.w3.org/2004/02/skos/core#> .
@prefix owl: <http://www.w3.org/2002/07/owl#> .
@prefix oa: <http://www.w3.org/ns/oa#> .
@prefix fabio: <http://purl.org/spar/fabio/> .

charme:doctypeScheme a skos:ConceptScheme ;
	skos:prefLabel "A SKOS Concept Scheme of document types for the CHARMe project"@en ;
	skos:definition "Document types are used to enforce a controlled vocabulary for CHARMe body and target elements and to facilitate search functions"@en ;
	dc:creator "Frank Kratzenstein" ;
	dc:contributor "Philip Kershaw" ;
	dc:created "2014-02-03" ;
	dc:modified "2014-11-28" ;
	owl:versionInfo "1.1" .

charme:DocType a owl:Class ;
	rdfs:label "The OWL class for the CHARMe technical document type specifications"@en .

charme:AlgorithmTheoreticalBasisDocument a skos:Concept, owl:Class ;
	skos:inScheme charme:doctypeScheme ;
	skos:prefLabel "Algorithm Theoretical Basis Document"@en ;
	skos:notation "ATBD"@en ;
	skos:broader fabio:TechnicalReport ;
	skos:definition "SKOS concept for Algorithm Theoretical Basis Document used for classifying CHARMe annotation bodies and targets."@en ;
	dc:created "2014-02-03" ;
	dc:modified "2014-11-28" ;
	owl:versionInfo "1.1" .

charme:ProductUserManual a skos:Concept, owl:Class ;
	skos:inScheme charme:doctypeScheme ;
	skos:prefLabel "Product User Manual"@en ;
	skos:notation "PUM"@en ;
	skos:broader fabio:TechnicalReport ;
	skos:definition "SKOS concept for Product User Manual used for classifying CHARMe annotation bodies and targets."@en ;
	dc:created "2014-02-03" ;
	dc:modified "2014-11-28" ;
	owl:versionInfo "1.1" .

charme:ValidationReport a skos:Concept, owl:Class ;
	skos:inScheme charme:doctypeScheme ;
	skos:prefLabel "Validation Report"@en ;
	skos:notation "VR"@en ;
	skos:broader fabio:TechnicalReport ;
	skos:definition "SKOS concept for Validation Report used for classifying CHARMe annotation bodies and targets."@en ;
	dc:created "2014-02-03" ;
	dc:modified "2014-11-28" ;
	owl:versionInfo "1.1" .

charme:OperationReport a skos:Concept, owl:Class ;
	skos:inScheme charme:doctypeScheme ;
	skos:prefLabel "Operation Report"@en ;
	skos:notation "OpR"@en ;
	skos:broader fabio:TechnicalReport ;
	skos:narrower charme:ServiceMessage ;
	skos:definition "SKOS concept for Operation Report used for classifying CHARMe annotation bodies and targets."@en ;
	dc:created "2014-02-03" ;
	dc:modified "2014-11-28" ;
	owl:versionInfo "1.1" .

charme:ServiceMessage a skos:Concept, owl:Class ;
	skos:inScheme charme:doctypeScheme ;
	skos:prefLabel "Service Message"@en ;
	skos:notation "SM"@en ;
	skos:broader charme:OperationReport ;
	skos:narrower charme:ProductChangeLog ;
	skos:narrower charme:KnownProductDisruption ;
	skos:definition "SKOS concept for Service Message used for classifying CHARMe annotation bodies and targets."@en ;
	dc:created "2014-02-03" ;
	dc:modified "2014-11-28" ;
	owl:versionInfo "1.1" .

charme:ProductChangeLog a skos:Concept, owl:Class ;
	skos:inScheme charme:doctypeScheme ;
	skos:prefLabel "Product Change Log"@en ;
	skos:notation "PCL"@en ;
	skos:broader charme:ServiceMessage  ;
	skos:definition "SKOS concept for Product Change Log used for classifying CHARMe annotation bodies and targets."@en ;
	dc:created "2014-02-03" ;
	dc:modified "2014-11-28" ;
	owl:versionInfo "1.1" .

charme:KnownProductDisruption a skos:Concept, owl:Class ;
	skos:inScheme charme:doctypeScheme ;
	skos:prefLabel "Known Product Disruption"@en ;
	skos:notation "KPD"@en ;
	skos:broader charme:ServiceMessage ;
	skos:definition "SKOS concept for Known Product Disruption used for classifying CHARMe annotation bodies and targets."@en ;
	dc:created "2014-02-03" ;
	dc:modified "2014-11-28" ;
	owl:versionInfo "1.1" .

# OWL relationships
charme:AlgorithmTheoreticalBasisDocument rdfs:subClassOf charme:DocType ;
	owl:disjointWith charme:ProductUserManual ;
	owl:disjointWith charme:ValidationReport ;
	owl:disjointWith charme:OperationReport ;
	owl:disjointWith charme:ServiceMessage ;
	owl:disjointWith charme:ProductChangeLog ;
	owl:disjointWith charme:KnownProductDisruption .

charme:ProductUserManual rdfs:subClassOf charme:DocType ;
	owl:disjointWith charme:AlgorithmTheoreticalBasisDocument ;
	owl:disjointWith charme:ValidationReport ;
	owl:disjointWith charme:OperationReport ;
	owl:disjointWith charme:ServiceMessage ;
	owl:disjointWith charme:ProductChangeLog ;
	owl:disjointWith charme:KnownProductDisruption .

charme:ValidationReport rdfs:subClassOf charme:DocType ;
	owl:disjointWith charme:AlgorithmTheoreticalBasisDocument ;
	owl:disjointWith charme:ProductUserManual ;
	owl:disjointWith charme:ServiceMessage ;
	owl:disjointWith charme:ProductChangeLog ;
	owl:disjointWith charme:KnownProductDisruption .

charme:OperationReport rdfs:subClassOf charme:DocType ;
	owl:disjointWith charme:AlgorithmTheoreticalBasisDocument ;
	owl:disjointWith charme:ProductUserManual ;
	owl:disjointWith charme:ValidationReport ;
	owl:disjointWith charme:ServiceMessage ;
	owl:disjointWith charme:ProductChangeLog ;
	owl:disjointWith charme:KnownProductDisruption .

charme:ServiceMessage rdfs:subClassOf charme:DocType ;
	owl:disjointWith charme:AlgorithmTheoreticalBasisDocument ;
	owl:disjointWith charme:ProductUserManual ;
	owl:disjointWith charme:ValidationReport ;
	owl:disjointWith charme:OperationReport ;
	owl:disjointWith charme:ProductChangeLog ;
	owl:disjointWith charme:KnownProductDisruption .

charme:ProductChangeLog rdfs:subClassOf charme:DocType ;
	owl:disjointWith charme:AlgorithmTheoreticalBasisDocument ;
	owl:disjointWith charme:ProductUserManual ;
	owl:disjointWith charme:ValidationReport ;
	owl:disjointWith charme:OperationReport ;
	owl:disjointWith charme:ServiceMessage ;
	owl:disjointWith charme:KnownProductDisruption .

charme:KnownProductDisruption rdfs:subClassOf charme:DocType ;
	owl:disjointWith charme:AlgorithmTheoreticalBasisDocument ;
	owl:disjointWith charme:ProductUserManual ;
	owl:disjointWith charme:ValidationReport ;
	owl:disjointWith charme:OperationReport ;
	owl:disjointWith charme:ServiceMessage ;
	owl:disjointWith charme:ProductChangeLog .
